almost finished determinism

src/vc0/progress.lean
@@ -396,17 +396,4 @@ begin
   case c0.state.ok.done : n { exact final state.final.done },
 end
 
-inductive io_equiv : io → state → io → state → Prop
-| none {s} : io_equiv none s none s
-| some {i o₁ o₂ s₁ s₂} : (o₁ = o₂ → s₁ = s₂) →
-  io_equiv (some (i, o₁)) s₁ (some (i, o₂)) s₂
-
-theorem determ {Γ : ast} (ok : Γ.ok) {s o₁ s₁ o₂ s₂}
-  (h₁ : step Γ s o₁ s₁) (h₂ : step Γ s o₂ s₂) : io_equiv o₁ s₁ o₂ s₂ :=
-sorry
-
-theorem determ' {Γ : ast} (ok : Γ.ok) {s o s₁ s₂}
-  (h₁ : step Γ s o s₁) (h₂ : step Γ s o s₂) : s₁ = s₂ :=
-by cases determ ok h₁ h₂; [refl, exact a rfl]
-
 end c0
